\section{Basics}
\subsection{Derivation rules}
\subsubsection{log(x)}
\begin{equation}
	\frac{\mathrm{d}}{\mathrm{d} x}\big( log(x) \big) = \frac{1}{x}
\end{equation}
\subsubsection{Chain rule}
\begin{equation}
	\frac{\mathrm{d}}{\mathrm{d} x}\big( f(g(x)) \big) = f'(g(x))*g'(x)
\end{equation}
Example:
\begin{equation}
	\frac{\mathrm{d}}{\mathrm{d} x}\big( log(1-\theta) \big) = \frac{1}{1-\theta}*-
	1
\end{equation}
Multiplication rule:
\begin{equation}
	\frac{\mathrm{d}}{\mathrm{d} x}\big( f(x)g(x) \big) = f'(x)*g(x) + f(x)*g'(x)
\end{equation}
\subsection{Matrix operations}
\subsubsection{Transpose rules}
\begin{equation}
	(AB)^{T}= B^{T}A^{T}
\end{equation}
Because $vector * Matrix * vector$ is a scalar
\begin{equation}
	w^{T}A^{T}y = y^{T}Aw
\end{equation}
\subsubsection{Matrix derivations}
\begin{equation}
	\begin{aligned}
		\Delta_{w}Aw = A^T\\ \Delta_w(w^{T}Aw) = 2Aw\\ \Delta_w(w^{T}w) = 2w\\
	\end{aligned}
\end{equation}